chore(library/init): remove `funext` and `quot` modules
The spaghetti initialization is almost over.

library/init/core.lean
@@ -1234,7 +1234,6 @@ theorem bool.ff_ne_tt : ff = tt → false
 def is_dec_eq {α : Sort u} (p : α → α → bool) : Prop   := ∀ ⦃x y : α⦄, p x y = tt → x = y
 def is_dec_refl {α : Sort u} (p : α → α → bool) : Prop := ∀ x, p x x = tt
 
-open decidable
 instance : decidable_eq bool
 | ff ff := is_true rfl
 | ff tt := is_false bool.ff_ne_tt
@@ -1259,7 +1258,7 @@ match (h a b) with
 | (is_false n₁) := proof_irrel n n₁ ▸ eq.refl (is_false n)
 end
 
-
+/- if-then-else expression theorems -/
 
 theorem if_pos {c : Prop} [h : decidable c] (hc : c) {α : Sort u} {t e : α} : (ite c t e) = t :=
 match h with
@@ -1770,3 +1769,308 @@ eq.subst (@iff_eq_eq a false) this
 theorem eq_true {a : Prop} : (a = true) = a :=
 have (a ↔ true) = a, from propext (iff_true a),
 eq.subst (@iff_eq_eq a true) this
+
+/- Quotients -/
+
+-- iff can now be used to do substitutions in a calculation
+@[subst] theorem iff_subst {a b : Prop} {p : Prop → Prop} (h₁ : a ↔ b) (h₂ : p a) : p b :=
+eq.subst (propext h₁) h₂
+
+namespace quot
+constant sound : Π {α : Sort u} {r : α → α → Prop} {a b : α}, r a b → quot.mk r a = quot.mk r b
+
+attribute [elab_as_eliminator] lift ind
+
+protected theorem lift_beta {α : Sort u} {r : α → α → Prop} {β : Sort v} (f : α → β) (c : ∀ a b, r a b → f a = f b) (a : α) : lift f c (quot.mk r a) = f a :=
+rfl
+
+protected theorem ind_beta {α : Sort u} {r : α → α → Prop} {β : quot r → Prop} (p : ∀ a, β (quot.mk r a)) (a : α) : (ind p (quot.mk r a) : β (quot.mk r a)) = p a :=
+rfl
+
+@[reducible, elab_as_eliminator]
+protected def lift_on {α : Sort u} {β : Sort v} {r : α → α → Prop} (q : quot r) (f : α → β) (c : ∀ a b, r a b → f a = f b) : β :=
+lift f c q
+
+@[elab_as_eliminator]
+protected theorem induction_on {α : Sort u} {r : α → α → Prop} {β : quot r → Prop} (q : quot r) (h : ∀ a, β (quot.mk r a)) : β q :=
+ind h q
+
+theorem exists_rep {α : Sort u} {r : α → α → Prop} (q : quot r) : ∃ a : α, (quot.mk r a) = q :=
+quot.induction_on q (λ a, ⟨a, rfl⟩)
+
+section
+variable {α : Sort u}
+variable {r : α → α → Prop}
+variable {β : quot r → Sort v}
+
+local notation `⟦`:max a `⟧` := quot.mk r a
+
+@[reducible]
+protected def indep (f : Π a, β ⟦a⟧) (a : α) : psigma β :=
+⟨⟦a⟧, f a⟩
+
+protected theorem indep_coherent (f : Π a, β ⟦a⟧)
+                     (h : ∀ (a b : α) (p : r a b), (eq.rec (f a) (sound p) : β ⟦b⟧) = f b)
+                     : ∀ a b, r a b → quot.indep f a = quot.indep f b  :=
+λ a b e, psigma.eq (sound e) (h a b e)
+
+protected theorem lift_indep_pr1
+  (f : Π a, β ⟦a⟧) (h : ∀ (a b : α) (p : r a b), (eq.rec (f a) (sound p) : β ⟦b⟧) = f b)
+  (q : quot r) : (lift (quot.indep f) (quot.indep_coherent f h) q).1 = q  :=
+quot.ind (λ (a : α), eq.refl (quot.indep f a).1) q
+
+@[reducible, elab_as_eliminator]
+protected def rec
+   (f : Π a, β ⟦a⟧) (h : ∀ (a b : α) (p : r a b), (eq.rec (f a) (sound p) : β ⟦b⟧) = f b)
+   (q : quot r) : β q :=
+eq.rec_on (quot.lift_indep_pr1 f h q) ((lift (quot.indep f) (quot.indep_coherent f h) q).2)
+
+@[reducible, elab_as_eliminator]
+protected def rec_on
+   (q : quot r) (f : Π a, β ⟦a⟧) (h : ∀ (a b : α) (p : r a b), (eq.rec (f a) (sound p) : β ⟦b⟧) = f b) : β q :=
+quot.rec f h q
+
+@[reducible, elab_as_eliminator]
+protected def rec_on_subsingleton
+   [h : ∀ a, subsingleton (β ⟦a⟧)] (q : quot r) (f : Π a, β ⟦a⟧) : β q :=
+quot.rec f (λ a b h, subsingleton.elim _ (f b)) q
+
+@[reducible, elab_as_eliminator]
+protected def hrec_on
+   (q : quot r) (f : Π a, β ⟦a⟧) (c : ∀ (a b : α) (p : r a b), f a == f b) : β q :=
+quot.rec_on q f
+  (λ a b p, eq_of_heq (calc
+    (eq.rec (f a) (sound p) : β ⟦b⟧) == f a : eq_rec_heq (sound p) (f a)
+                                 ... == f b : c a b p))
+end
+end quot
+
+def quotient {α : Sort u} (s : setoid α) :=
+@quot α setoid.r
+
+namespace quotient
+
+protected def mk {α : Sort u} [s : setoid α] (a : α) : quotient s :=
+quot.mk setoid.r a
+
+notation `⟦`:max a `⟧`:0 := quotient.mk a
+
+def sound {α : Sort u} [s : setoid α] {a b : α} : a ≈ b → ⟦a⟧ = ⟦b⟧ :=
+quot.sound
+
+@[reducible, elab_as_eliminator]
+protected def lift {α : Sort u} {β : Sort v} [s : setoid α] (f : α → β) : (∀ a b, a ≈ b → f a = f b) → quotient s → β :=
+quot.lift f
+
+@[elab_as_eliminator]
+protected theorem ind {α : Sort u} [s : setoid α] {β : quotient s → Prop} : (∀ a, β ⟦a⟧) → ∀ q, β q :=
+quot.ind
+
+@[reducible, elab_as_eliminator]
+protected def lift_on {α : Sort u} {β : Sort v} [s : setoid α] (q : quotient s) (f : α → β) (c : ∀ a b, a ≈ b → f a = f b) : β :=
+quot.lift_on q f c
+
+@[elab_as_eliminator]
+protected theorem induction_on {α : Sort u} [s : setoid α] {β : quotient s → Prop} (q : quotient s) (h : ∀ a, β ⟦a⟧) : β q :=
+quot.induction_on q h
+
+theorem exists_rep {α : Sort u} [s : setoid α] (q : quotient s) : ∃ a : α, ⟦a⟧ = q :=
+quot.exists_rep q
+
+section
+variable {α : Sort u}
+variable [s : setoid α]
+variable {β : quotient s → Sort v}
+
+protected def rec
+   (f : Π a, β ⟦a⟧) (h : ∀ (a b : α) (p : a ≈ b), (eq.rec (f a) (quotient.sound p) : β ⟦b⟧) = f b)
+   (q : quotient s) : β q :=
+quot.rec f h q
+
+@[reducible, elab_as_eliminator]
+protected def rec_on
+   (q : quotient s) (f : Π a, β ⟦a⟧) (h : ∀ (a b : α) (p : a ≈ b), (eq.rec (f a) (quotient.sound p) : β ⟦b⟧) = f b) : β q :=
+quot.rec_on q f h
+
+@[reducible, elab_as_eliminator]
+protected def rec_on_subsingleton
+   [h : ∀ a, subsingleton (β ⟦a⟧)] (q : quotient s) (f : Π a, β ⟦a⟧) : β q :=
+@quot.rec_on_subsingleton _ _ _ h q f
+
+@[reducible, elab_as_eliminator]
+protected def hrec_on
+   (q : quotient s) (f : Π a, β ⟦a⟧) (c : ∀ (a b : α) (p : a ≈ b), f a == f b) : β q :=
+quot.hrec_on q f c
+end
+
+section
+universes u_a u_b u_c
+variables {α : Sort u_a} {β : Sort u_b} {φ : Sort u_c}
+variables [s₁ : setoid α] [s₂ : setoid β]
+include s₁ s₂
+
+@[reducible, elab_as_eliminator]
+protected def lift₂
+   (f : α → β → φ)(c : ∀ a₁ a₂ b₁ b₂, a₁ ≈ b₁ → a₂ ≈ b₂ → f a₁ a₂ = f b₁ b₂)
+   (q₁ : quotient s₁) (q₂ : quotient s₂) : φ :=
+quotient.lift
+  (λ (a₁ : α), quotient.lift (f a₁) (λ (a b : β), c a₁ a a₁ b (setoid.refl a₁)) q₂)
+  (λ (a b : α) (h : a ≈ b),
+     @quotient.ind β s₂
+       (λ (a_1 : quotient s₂),
+          (quotient.lift (f a) (λ (a_1 b : β), c a a_1 a b (setoid.refl a)) a_1)
+          =
+          (quotient.lift (f b) (λ (a b_1 : β), c b a b b_1 (setoid.refl b)) a_1))
+       (λ (a' : β), c a a' b a' h (setoid.refl a'))
+       q₂)
+  q₁
+
+@[reducible, elab_as_eliminator]
+protected def lift_on₂
+  (q₁ : quotient s₁) (q₂ : quotient s₂) (f : α → β → φ) (c : ∀ a₁ a₂ b₁ b₂, a₁ ≈ b₁ → a₂ ≈ b₂ → f a₁ a₂ = f b₁ b₂) : φ :=
+quotient.lift₂ f c q₁ q₂
+
+@[elab_as_eliminator]
+protected theorem ind₂ {φ : quotient s₁ → quotient s₂ → Prop} (h : ∀ a b, φ ⟦a⟧ ⟦b⟧) (q₁ : quotient s₁) (q₂ : quotient s₂) : φ q₁ q₂ :=
+quotient.ind (λ a₁, quotient.ind (λ a₂, h a₁ a₂) q₂) q₁
+
+@[elab_as_eliminator]
+protected theorem induction_on₂
+   {φ : quotient s₁ → quotient s₂ → Prop} (q₁ : quotient s₁) (q₂ : quotient s₂) (h : ∀ a b, φ ⟦a⟧ ⟦b⟧) : φ q₁ q₂ :=
+quotient.ind (λ a₁, quotient.ind (λ a₂, h a₁ a₂) q₂) q₁
+
+@[elab_as_eliminator]
+protected theorem induction_on₃
+   [s₃ : setoid φ]
+   {δ : quotient s₁ → quotient s₂ → quotient s₃ → Prop} (q₁ : quotient s₁) (q₂ : quotient s₂) (q₃ : quotient s₃) (h : ∀ a b c, δ ⟦a⟧ ⟦b⟧ ⟦c⟧)
+   : δ q₁ q₂ q₃ :=
+quotient.ind (λ a₁, quotient.ind (λ a₂, quotient.ind (λ a₃, h a₁ a₂ a₃) q₃) q₂) q₁
+end
+
+section exact
+variable   {α : Sort u}
+variable   [s : setoid α]
+include s
+
+private def rel (q₁ q₂ : quotient s) : Prop :=
+quotient.lift_on₂ q₁ q₂
+  (λ a₁ a₂, a₁ ≈ a₂)
+  (λ a₁ a₂ b₁ b₂ a₁b₁ a₂b₂,
+    propext (iff.intro
+      (λ a₁a₂, setoid.trans (setoid.symm a₁b₁) (setoid.trans a₁a₂ a₂b₂))
+      (λ b₁b₂, setoid.trans a₁b₁ (setoid.trans b₁b₂ (setoid.symm a₂b₂)))))
+
+local infix `~` := rel
+
+private theorem rel.refl : ∀ q : quotient s, q ~ q :=
+λ q, quot.induction_on q (λ a, setoid.refl a)
+
+private theorem eq_imp_rel {q₁ q₂ : quotient s} : q₁ = q₂ → q₁ ~ q₂ :=
+assume h, eq.rec_on h (rel.refl q₁)
+
+theorem exact {a b : α} : ⟦a⟧ = ⟦b⟧ → a ≈ b :=
+assume h, eq_imp_rel h
+end exact
+
+section
+universes u_a u_b u_c
+variables {α : Sort u_a} {β : Sort u_b}
+variables [s₁ : setoid α] [s₂ : setoid β]
+include s₁ s₂
+
+@[reducible, elab_as_eliminator]
+protected def rec_on_subsingleton₂
+   {φ : quotient s₁ → quotient s₂ → Sort u_c} [h : ∀ a b, subsingleton (φ ⟦a⟧ ⟦b⟧)]
+   (q₁ : quotient s₁) (q₂ : quotient s₂) (f : Π a b, φ ⟦a⟧ ⟦b⟧) : φ q₁ q₂:=
+@quotient.rec_on_subsingleton _ s₁ (λ q, φ q q₂) (λ a, quotient.ind (λ b, h a b) q₂) q₁
+  (λ a, quotient.rec_on_subsingleton q₂ (λ b, f a b))
+
+end
+end quotient
+
+section
+variable {α : Type u}
+variable (r : α → α → Prop)
+
+inductive eqv_gen : α → α → Prop
+| rel {} : Π x y, r x y → eqv_gen x y
+| refl {} : Π x, eqv_gen x x
+| symm {} : Π x y, eqv_gen x y → eqv_gen y x
+| trans {} : Π x y z, eqv_gen x y → eqv_gen y z → eqv_gen x z
+
+theorem eqv_gen.is_equivalence : equivalence (@eqv_gen α r) :=
+mk_equivalence _ eqv_gen.refl eqv_gen.symm eqv_gen.trans
+
+def eqv_gen.setoid : setoid α :=
+setoid.mk _ (eqv_gen.is_equivalence r)
+
+theorem quot.exact {a b : α} (H : quot.mk r a = quot.mk r b) : eqv_gen r a b :=
+@quotient.exact _ (eqv_gen.setoid r) a b (@congr_arg _ _ _ _
+  (quot.lift (@quotient.mk _ (eqv_gen.setoid r)) (λx y h, quot.sound (eqv_gen.rel x y h))) H)
+
+theorem quot.eqv_gen_sound {r : α → α → Prop} {a b : α} (H : eqv_gen r a b) : quot.mk r a = quot.mk r b :=
+eqv_gen.rec_on H
+  (λ x y h, quot.sound h)
+  (λ x, rfl)
+  (λ x y _ IH, eq.symm IH)
+  (λ x y z _ _ IH₁ IH₂, eq.trans IH₁ IH₂)
+end
+
+instance {α : Sort u} {s : setoid α} [d : ∀ a b : α, decidable (a ≈ b)] : decidable_eq (quotient s) :=
+λ q₁ q₂ : quotient s,
+  quotient.rec_on_subsingleton₂ q₁ q₂
+    (λ a₁ a₂,
+      match (d a₁ a₂) with
+      | (is_true h₁)  := is_true (quotient.sound h₁)
+      | (is_false h₂) := is_false (λ h, absurd (quotient.exact h) h₂)
+      end)
+
+/- Function extensionality -/
+
+namespace function
+variables {α : Sort u} {β : α → Sort v}
+
+protected def equiv (f₁ f₂ : Π x : α, β x) : Prop := ∀ x, f₁ x = f₂ x
+
+local infix `~` := function.equiv
+
+protected theorem equiv.refl (f : Π x : α, β x) : f ~ f := assume x, rfl
+
+protected theorem equiv.symm {f₁ f₂ : Π x: α, β x} : f₁ ~ f₂ → f₂ ~ f₁ :=
+λ h x, eq.symm (h x)
+
+protected theorem equiv.trans {f₁ f₂ f₃ : Π x: α, β x} : f₁ ~ f₂ → f₂ ~ f₃ → f₁ ~ f₃ :=
+λ h₁ h₂ x, eq.trans (h₁ x) (h₂ x)
+
+protected theorem equiv.is_equivalence (α : Sort u) (β : α → Sort v) : equivalence (@function.equiv α β) :=
+mk_equivalence (@function.equiv α β) (@equiv.refl α β) (@equiv.symm α β) (@equiv.trans α β)
+end function
+
+section
+open quotient
+variables {α : Sort u} {β : α → Sort v}
+
+@[instance]
+private def fun_setoid (α : Sort u) (β : α → Sort v) : setoid (Π x : α, β x) :=
+setoid.mk (@function.equiv α β) (function.equiv.is_equivalence α β)
+
+private def extfun (α : Sort u) (β : α → Sort v) : Sort (imax u v) :=
+quotient (fun_setoid α β)
+
+private def fun_to_extfun (f : Π x : α, β x) : extfun α β :=
+⟦f⟧
+private def extfun_app (f : extfun α β) : Π x : α, β x :=
+assume x,
+quot.lift_on f
+  (λ f : Π x : α, β x, f x)
+  (λ f₁ f₂ h, h x)
+
+theorem funext {f₁ f₂ : Π x : α, β x} (h : ∀ x, f₁ x = f₂ x) : f₁ = f₂ :=
+show extfun_app ⟦f₁⟧ = extfun_app ⟦f₂⟧, from
+congr_arg extfun_app (sound h)
+end
+
+local infix `~` := function.equiv
+
+instance pi.subsingleton {α : Sort u} {β : α → Sort v} [∀ a, subsingleton (β a)] : subsingleton (Π a, β a) :=
+⟨λ f₁ f₂, funext (λ a, subsingleton.elim (f₁ a) (f₂ a))⟩
