library/init/classical.lean
@@ -4,7 +4,7 @@ Released under Apache 2.0 license as described in the file LICENSE.
 Authors: Leonardo de Moura, Jeremy Avigad, Mario Carneiro
 -/
 prelude
-import init.funext
+import init.core
 
 namespace classical
 universes u v
